\documentclass[twoside,11pt]{homework}

\usepackage{dsfont}
\usepackage{amsmath}
\usepackage{graphicx}

\coursename{COMS 4771 Machine Learning (Spring 2020)} 

\studname{Angela Wang}     
\studmail{aw3062@columbia.edu}
\hwNo{1}      
\date{02/21/2020}  
\begin{document}
\maketitle



\section*{Problem 3} 
\subsection*{(i)}
\subsection*{(ii)}
\subsection*{(iii)}


\section*{Problem 4} 
\subsection*{(i)}
	\begin{proof}
		Since $M^{T} = (A^{T}A)^{T} = A^{T}A = M$, M is symmetric. 
		For any column vector $z\in \mathbb{R}^d$, $z^TMz = z^TA^TAz = (Az)^T (Az) = (Az)\cdot(Az) \geq 0$, 
		so M is positive semi-definite.
	\end{proof}
\subsection*{(ii)}
	\begin{proof}
		Base case: if $N=1$, then by definition, 
		\begin{align*}
			\beta^{(1)} &= \beta^{(0)}+ \eta  A^{T} (b-A \beta^{(0)}) \\
			&= \eta v - \eta M \beta^{(0)} \\
			&= \eta v 
		\end{align*}
		Assuming the statement $\beta^{(N)} = \eta \sum_{k=0}^{N-1} (I-\eta M)^k v$ is true for $N=n$, then for $N=n+1$ we have
		\begin{align*}
			\beta^{(n+1)} &= (I-\eta M) \beta^{(n)} + \eta v \tag{definition} \\
			&= (I-\eta M) \eta  \sum_{k=0}^{n-1} (I-\eta M)^k v + \eta v \tag{induction hypothesis} \\
			&= \eta  \sum_{k=0}^{n-1} (I-\eta M)^{(k+1)} v + \eta (I-\eta M)^0 v \\
			&= \eta  \sum_{k=1}^{n} (I-\eta M)^{(k)} v + \eta (I-\eta M)^0 v \\
			&= \eta  \sum_{k=0}^{n} (I-\eta M)^{(k)} v
		\end{align*}
	\end{proof}
\subsection*{(iii)}
	Since $M$ is a real symmetric matrix, it has a decomposition $M = P D P^{-1}$, 
	where $P$ is a matrix composed of orthogonal eigenvectors corresponding to distinct eigenvalues,
	and $D:= \text{diag}(\lambda_1,\dots, \lambda_d)$.
	\begin{align*}
		&\eta \sum_{k=0}^{N-1} (I-\eta M)^k \\
		=& \eta \sum_{k=0}^{N-1} \sum_{i=0}^{k} I^{k-i}(-\eta M)^i \\
		=&  \sum_{k=0}^{N-1} \sum_{i=0}^{k} (-1)^i\eta^{i+1} M^{i} \\
		=&  \sum_{k=0}^{N-1} \sum_{i=0}^{k} (-1)^i\eta^{i+1} PD^{i}P^{-1} \\
		=& P  \left(\sum_{k=0}^{N-1} \sum_{i=0}^{k}  (-1)^i\eta^{i+1}  \text{diag}(\lambda_1^i,\dots, \lambda_d^i) \right) P^{-1} \\
		=& P \, \text{diag} \left(\sum_{k=0}^{N-1} \sum_{i=0}^{k}  (-1)^i\eta^{i+1} \lambda_1^i,\dots, 
		\sum_{k=0}^{N-1} \sum_{i=0}^{k}  (-1)^i\eta^{i+1} \lambda_d^i \right)  P^{-1}\\
		=& P \, \text{diag} \left(
			\sum_{i=0}^{N-1} (N-i) (-1)^{i}\eta^{i+1}\lambda^i_1
			\dots, 
			\sum_{i=0}^{N-1} (N-i) (-1)^{i}\eta^{i+1}\lambda^i_d
		\right)  P^{-1}
	\end{align*}
	Since $I$, $M$ are symmetric, $\eta \sum_{k=0}^{N-1} (I-\eta M)^k$ is symmetric, 
	and its eiganvalues $\lambda_1',\dots, \lambda_d'$ are given by
	\begin{align*}
		\lambda_j' = \sum_{i=0}^{N-1} (N-i) (-1)^{i}\eta^{i+1}\lambda^i_j
	\end{align*}
	for any $j=1,\dots,d$.
\subsection*{(iv)}



\end{document} 
